Phi_Min.thy
@@ -312,7 +312,7 @@ lemma [\<phi>reason 1200 on \<open>PROP Branch_Convergence_Type_Pattern (Var ?v 
   \<open> PROP Branch_Convergence_Type_Pattern (Var v T) (Var v T')\<close>
   unfolding Branch_Convergence_Type_Pattern_def ..
 
-lemma [\<phi>reason 1200 on \<open>\<^bold>v\<^bold>i\<^bold>e\<^bold>w ?R \<heavy_comma> ?H \<longmapsto> ?R''' * \<blangle> ?x \<Ztypecolon> Var ?var ?T \<brangle> \<^bold>w\<^bold>i\<^bold>t\<^bold>h ?P \<^bold>@\<^bold>G\<^bold>O\<^bold>A\<^bold>L ?G\<close>]:
+lemma [\<phi>reason 1500 on \<open>\<^bold>v\<^bold>i\<^bold>e\<^bold>w ?R \<heavy_comma> ?H \<longmapsto> ?R''' * \<blangle> ?x \<Ztypecolon> Var ?var ?T \<brangle> \<^bold>w\<^bold>i\<^bold>t\<^bold>h ?P \<^bold>@\<^bold>G\<^bold>O\<^bold>A\<^bold>L ?G\<close>]:
     \<comment> \<open>attempts the immediate cell\<close>
   " CHK_SUBGOAL G
 \<Longrightarrow> x \<Ztypecolon> T \<^bold>i\<^bold>m\<^bold>p\<^bold>l\<^bold>i\<^bold>e\<^bold>s x' \<Ztypecolon> T' \<^bold>a\<^bold>n\<^bold>d P
@@ -320,7 +320,7 @@ lemma [\<phi>reason 1200 on \<open>\<^bold>v\<^bold>i\<^bold>e\<^bold>w ?R \<hea
   unfolding GOAL_CTXT_def FOCUS_TAG_def
   by (simp add: Var_view_shift \<phi>frame_view)
 
-lemma [\<phi>reason 1100 on \<open>\<^bold>v\<^bold>i\<^bold>e\<^bold>w ?R \<heavy_comma> ?H \<longmapsto> ?R''' * \<blangle> ?x \<Ztypecolon> Var ?var ?T \<brangle> \<^bold>w\<^bold>i\<^bold>t\<^bold>h ?P \<^bold>@\<^bold>G\<^bold>O\<^bold>A\<^bold>L ?G\<close>]:
+lemma [\<phi>reason 1450 on \<open>\<^bold>v\<^bold>i\<^bold>e\<^bold>w ?R \<heavy_comma> ?H \<longmapsto> ?R''' * \<blangle> ?x \<Ztypecolon> Var ?var ?T \<brangle> \<^bold>w\<^bold>i\<^bold>t\<^bold>h ?P \<^bold>@\<^bold>G\<^bold>O\<^bold>A\<^bold>L ?G\<close>]:
   \<open> \<^bold>v\<^bold>i\<^bold>e\<^bold>w R \<longmapsto> R' \<heavy_comma> \<blangle> x \<Ztypecolon> Var var T \<brangle> \<^bold>w\<^bold>i\<^bold>t\<^bold>h P  \<^bold>@\<^bold>G\<^bold>O\<^bold>A\<^bold>L G
 \<Longrightarrow> \<^bold>v\<^bold>i\<^bold>e\<^bold>w R \<heavy_comma> H \<longmapsto> R' \<heavy_comma> H \<heavy_comma> \<blangle> x \<Ztypecolon> Var var T \<brangle> \<^bold>w\<^bold>i\<^bold>t\<^bold>h P  \<^bold>@\<^bold>G\<^bold>O\<^bold>A\<^bold>L G\<close>
   using assertion_level_reasoning_skip[OF CHK_SUBGOAL_I] .
@@ -384,9 +384,9 @@ definition op_const_size_t :: "nat \<Rightarrow> ('VAL,'VAL,'RES_N,'RES) proc"
 
 definition op_add :: "nat \<Rightarrow> ('VAL \<times> 'VAL, 'VAL, 'VAL, 'RES_N, 'RES) proc'"
   where "op_add bits =
-      \<phi>M_caseV (\<lambda>va vb.
-      \<phi>M_getV (\<tau>Int bits) (snd o V_int.dest) va (\<lambda>val_a.
+      \<phi>M_caseV (\<lambda>vb va.
       \<phi>M_getV (\<tau>Int bits) (snd o V_int.dest) vb (\<lambda>val_b.
+      \<phi>M_getV (\<tau>Int bits) (snd o V_int.dest) va (\<lambda>val_a.
       Return (sem_value (V_int.mk (bits, ((val_a + val_b) mod 2^bits))))
   )))"
 
